deserialization demo

jsonstar/JsonStar.Json.fst
@@ -1,5 +1,7 @@
 ﻿module JsonStar.Json
 
+open FStar.Pervasives.Native
+
 let addProp (key:string) (v:json) (j:json{JObject? j}) : Tot (r:json{JObject? r}) =
     JObject ((key, v) :: (JObject?.props j))
 
@@ -7,3 +9,24 @@ let addPropOpt (key:string) (vo:option json) (j:json{JObject? j}) : Tot (r:json{
     match vo with
     | Some v -> addProp key v j
     | None -> j
+
+// NOTE: There's some mismatch between the option type produced with extracted find from 
+// FStar.List.Tot and option used in this file to pattern match. By copying the definition of find
+// I can work around this for now. 
+val find: #a:Type
+        -> f:(a -> Tot bool)
+        -> list a
+        -> Tot (option (x:a{f x}))
+let rec find #a f l = match l with
+  | [] -> None #(x:a{f x}) //These type annotations are only present because it makes bootstrapping go much faster
+  | hd::tl -> if f hd then Some #(x:a{f x}) hd else find f tl
+
+let getProp (key : string) (j:json{JObject? j}) : Tot (option json) =
+    let props = JObject?.props j in
+    let prop_opt = find (fun (k,_) -> k = key) props in
+    match prop_opt with
+    | Some prop -> begin
+        let (_, v) = prop in
+        Some v
+        end
+    | None -> None
