JsonStar.Serialization.Demo/JsonStar.Serialization.Demo3.fst
@@ -1,0 +1,198 @@
+module JsonStar.Serialization.Demo3
+
+open JsonStar.Json
+open FStar.Tactics
+open FStar.Tactics.Typeclasses
+
+module P = FStar.Printf
+module LessInterestingHelpers = JsonStar.Schema.Generation.Reader
+module Helpers = JsonStar.Schema.Generation.Helpers
+
+type result (a : Type) = 
+    | Error of string
+    | Valid of a
+    
+[@@ noextract_to "FSharp"]
+let is_record_type (e : env) (typ : term) : Tac bool = 
+    match inspect typ with
+    | Tv_FVar fv -> 
+        // This is just more pattern matching on term representation to see if 
+        // 'typ' represents a record type (which is a discriminated union with a single constructor called 'Mk{record_type_name}')
+        LessInterestingHelpers.isRecord e fv
+    | _ -> false
+
+// Adds "Mk" to last segment of the qualified name
+[@@ noextract_to "FSharp"]
+let rec record_constructor_name (n : list string{Cons? n}) : Tot (list string) = 
+    match n with
+    | [ x ] -> [ "Mk" ^ x ]
+    | x :: xs -> x :: record_constructor_name xs
+
+[@@ noextract_to "FSharp"]
+let typ_to_string (x : typ) : Tac (n : list string{Cons? n}) = 
+    match inspect x with
+    | Tv_FVar fv -> begin
+        match inspect_fv fv with
+        | [] -> fail "Type name can't be empty"
+        | n -> n
+        end
+    | _ -> fail "Can't extract typename from typ"
+
+[@@ noextract_to "FSharp"]
+let call (f : term) (arg : term) : Tac term = pack (Tv_App f (arg, Q_Explicit))
+
+[@@ noextract_to "FSharp"]
+let drop_b2t (t : term) : Tac term = 
+    match inspect t with
+    | Tv_App f (arg, _) -> begin 
+        if Helpers.termeq f (`Prims.b2t)
+            then arg
+            else t
+        end
+    | _ -> t
+
+[@@ noextract_to "FSharp"]
+let mk_function (b : binder) (body : term) = pack (Tv_Abs b body)
+
+[@@ noextract_to "FSharp"]
+let create_deserializer_f (e : env) (t : Type) (json_arg_binder : binder) : Tac term = 
+    let real_arg = pack (Tv_Var (bv_of_binder json_arg_binder)) in
+
+    let qname = typ_to_string (quote t) in
+    let ctr_name = record_constructor_name qname in
+
+    let s = lookup_typ e qname in
+    match s with
+    | Some s -> begin
+        match inspect_sigelt s with
+        | Sg_Inductive _ _ _ _ cts -> begin
+            if List.Tot.length cts = 1
+                then begin
+                    // We can assume that cts is a single-element list as we've checked that with 'is_record_type'
+                    let ctr = snd (List.Tot.hd cts) in
+
+                    match inspect ctr with
+                    | Tv_Arrow bi _ -> begin
+                        // TODO: Just a single field for now
+                        let (b, _) = inspect_binder bi in
+                        let bvv = inspect_bv b in
+                        let prop_name = bvv.bv_ppname in
+                        let prop_type = bvv.bv_sort in
+                        let prop_refinement_fun = 
+                            match inspect prop_type with
+                            | Tv_Refine b phi -> begin
+                                mk_function (pack_binder b Q_Explicit []) (drop_b2t phi)
+                                end
+                            | _ -> fail "Unsupported prop-type"
+                        in
+
+                        let prop_json_option_term = call (call (quote JsonStar.Json.getProp) (quote prop_name)) real_arg in 
+
+                        let ctr_callable_term = (mk_function bi (call (pack (Tv_FVar (pack_fv ctr_name))) (pack (Tv_Var b)))) in
+
+                        let match_json = 
+                            `(fun (prop_j:option json) ->
+                                match prop_j with
+                                | Some p -> begin
+                                    match p with
+                                    | JNumber num JInt -> begin 
+                                        let num_v = JsonStar.Parser.int_of_string num in
+                                        let prop_ref : int -> bool = `#prop_refinement_fun in
+                                        if prop_ref num_v 
+                                            then Valid ((`#ctr_callable_term) num_v)
+                                            else Error "BBB"
+                                        end
+                                    | JString s -> Error (P.sprintf "Value string: %s" s)
+                                    | JBoolean b -> Error (P.sprintf "Value bool: %b" b)
+                                    | _ -> Error "Unsupported value"
+                                    end
+                                | _ -> Error (P.sprintf "Unsupported value type")
+                            )
+                        in
+                        let body = call match_json prop_json_option_term in
+                        let final = mk_function json_arg_binder body in
+
+                        final
+                       end
+                    | _ -> fail "Not implemented yet"
+                    end
+                else fail (P.sprintf "Expected record type '%s' to have a single constructor." (implode_qn qname))
+            end
+        | _ -> fail (P.sprintf "Expected record, got %s" (term_to_string (pack (Tv_FVar (pack_fv qname)))))
+        end
+    | None -> fail (P.sprintf "Could not find type %s" (implode_qn qname))
+
+/////////// Function generation part end
+
+// This has to produce a function: (json -> result t)
+// Note the usage of 'fail' for typechecking time errors (when we're dealing with bad usage or unsupported kinds of typ_term as the 
+// structure of the type to deserialize is known during typechecking)
+[@@ noextract_to "FSharp"]
+let deserialize_impl (t : Type) (typ_term : term) : Tac unit = 
+    let e = cur_env() in
+    match inspect (cur_goal ()) with
+    | Tv_Arrow b c -> begin
+        if is_record_type e typ_term
+            then begin
+                let deserializer_f = create_deserializer_f e t b in
+                exact deserializer_f
+                end
+            else fail "We only support deserialization of a record, sorry!"
+        end
+    | _ -> fail "Invalid usage of deserialize_impl_dyn. It should be used to generate a function: 'json -> result t'"
+
+
+class serializable a = {
+    //serialize_gen: a -> result json; 
+    deserialize_gen: (j:json{JObject? j}) -> result a
+}
+
+//let serialize   #a {| serializable a |} v = serialize_gen   #a v
+let deserialize #a {| serializable a |} v = deserialize_gen #a v
+
+/// Example record type that we would want to deserialize //
+type r =                                                  //
+    {                                                     //
+        l : x:int{x >= 5};                                //
+    }                                                     //
+////////////////////////////////////////////////////////////
+
+// NOTE1: 
+//     We can't inspect type at runtime with F*, so we need some boilerplate to 
+//     have a nice, generic serialization function. For each type we need to define an instance of 
+//     a type class.
+// NOTE2: 
+//     Unfortunately we can't simply pass json argument to 'deserialize_impl' and pattern match on it. 
+//     We actually need to produce a function type with Meta-F* that takes a json argument and does something with it. 
+instance r_serializable: serializable r = {
+   //serialize_gen = (fun x -> synth_by_tactic (fun () -> serialize_impl (`r) x));
+   deserialize_gen = synth_by_tactic (fun () -> deserialize_impl r (`r));
+}
+
+// We could simplify it a little and generate these instances with a line similar to the following:
+// %splice[] (generate_serializable (`r))
+// where generate_serializable is a Meta-F* function that realizes the type class instance. 
+// Still it's an extra line per type to make it json-serializable. 
+// The good part is that we should be able to add these instances on top of library types as long 
+// as their definition is visible/accessible. 
+
+    
+let process_r_from_json (j : json{JObject? j}) : Tot (result (x:int{x >= 5})) = 
+    let r_deserialized : result r = deserialize j in
+    match r_deserialized with
+    | Valid rv -> Valid rv.l
+    | Error msg -> Error msg
+
+let main = 
+    FStar.IO.print_string "Write json:\n";
+    let json_str = FStar.IO.input_line () in
+    let json = JsonStar.Parser.parse json_str in
+    if JObject? json
+        then begin
+            let l_r = process_r_from_json json in
+            match l_r with
+            | Valid l -> FStar.IO.print_string (P.sprintf "Value of l field is: %d\n" l)
+            | Error msg -> FStar.IO.print_string (P.sprintf "Value of l field is not available due to: %s\n" msg)
+            end
+        else FStar.IO.print_string "Provided json does not represent an object\n"
+    
