jsonstar/JsonStar.Parser.fsti
@@ -1,7 +1,9 @@
-module JsonStar_Parser
+module JsonStar.Parser
 open FStar.All
 open JsonStar.Json
 
 /// Attempts to parse a provided json. Throws an exception if the json is incorrect. 
 /// NOTE: This is currently implemented with unverified F# code under the cover.
 val parse : string -> ML json
+
+val int_of_string : string -> Tot int
